src/verification/BlockVer/BootcodeBlocks.v
@@ -27,7 +27,7 @@ Import ListNotations.
 Import asn.notations.
 Import Erasure.notations.
 
-Module Bootcode.
+Module BootcodeBlocks.
   Import Utils.
 
   Definition asn_ipe_registers_init {Σ} : Assertion Σ :=
@@ -79,10 +79,10 @@ Module Bootcode.
   Local Ltac symbolic_simpl :=
     vm_compute; constructor; simpl.
 
-  Definition asn_init_pc {Σ} (pc : Term _ ty.Address) : Assertion (Σ ▻ "a" :: ty.Address) :=
-    term_var "a" = pc.
-  Definition asn_fin_pc {Σ} (pc : Term _ ty.Address) : Assertion (Σ ▻ "an" :: ty.Address) :=
-    term_var "an" = pc.
+  Definition asn_init_pc {Σ} (pc : bv 16) : Assertion (Σ ▻ "a" :: ty.Address) :=
+    term_var "a" = term_val ty.Address pc.
+  Definition asn_fin_pc {Σ} (pc : bv 16) : Assertion (Σ ▻ "an" :: ty.Address) :=
+    term_var "an" = term_val ty.Address pc.
 
   Local Notation "v -' n" :=
     (term_binop bop.bvsub v (term_val ty.wordBits [bv n]))
@@ -91,26 +91,43 @@ Module Bootcode.
   Definition asn_byte_zero {Σ} (b : Term Σ ty.byteBits) : Assertion Σ :=
     b = term_val ty.byteBits [bv 0].
 
-  Definition saved_ptr {Σ} : Term Σ _ := term_val ty.Address [bv 0x4200].
-  Definition isp {Σ} : Term Σ _ := term_val ty.Address [bv 0x4202].
+  Definition saved_ptr_bv : bv 16 := [bv 0x4200].
+  Definition isp_bv : bv 16 := [bv 0x4202].
+  Definition saved_ptr {Σ} : Term Σ _ := term_val ty.Address saved_ptr_bv.
+  Definition isp {Σ} : Term Σ _ := term_val ty.Address isp_bv.
 
   Definition byte_zero {Σ} : Term Σ _ := term_val ty.byteBits [bv 0].
 
-  Definition valid_flag {Σ} : Term Σ _ := term_val ty.wordBits [bv 0xAAAA].
-  Definition ipe_sig_valid_src {Σ} : Term Σ _ := term_val ty.Address [bv 0xFF88].
-  Definition ipe_struct_pointer_src {Σ} : Term Σ _ := term_val ty.Address [bv 0xFF8A].
 
-  Definition start_bootcode_start{Σ} : Term Σ _ := term_val ty.wordBits [bv 0].
-  Definition transfer_if_valid_struct_start {Σ} : Term Σ _ := term_val ty.wordBits [bv 0x4].
-  Definition check_struct_start {Σ} : Term Σ _ := term_val ty.wordBits [bv 0xC].
-  Definition evaluate_struct_start {Σ} : Term Σ _ := term_val ty.wordBits [bv 0x1A].
-  Definition mass_erase_start {Σ} : Term Σ _ := term_val ty.wordBits [bv 0x2E].
-  Definition end_addr {Σ} : Term Σ _ := term_val ty.wordBits [bv 0x100].
+  Definition valid_flag_bv : bv 16 := [bv 0xAAAA].
+  Definition ipe_sig_valid_src_bv : bv 16 := [bv 0xFF88].
+  Definition ipe_struct_pointer_src_bv : bv 16 := [bv 0xFF8A].
+  Definition valid_flag {Σ} : Term Σ _ := term_val ty.wordBits valid_flag_bv.
+  Definition ipe_sig_valid_src {Σ} : Term Σ _ := term_val ty.Address ipe_sig_valid_src_bv.
+  Definition ipe_struct_pointer_src {Σ} : Term Σ _ := term_val ty.Address ipe_struct_pointer_src_bv.
+
+  Definition start_bootcode_start : bv 16 := [bv 0].
+  Definition transfer_if_valid_struct_start : bv 16 := [bv 0x4].
+  Definition check_struct_start : bv 16 := [bv 0xC].
+  Definition evaluate_struct_start : bv 16 := [bv 0x1A].
+  Definition mass_erase_start : bv 16 := [bv 0x2E].
+  Definition end_addr : bv 16 := [bv 0x3A].
+
+  Definition start_bootcode_size := Z.to_nat (bv.unsigned (transfer_if_valid_struct_start - start_bootcode_start)).
+  Definition transfer_if_valid_struct_size := Z.to_nat (bv.unsigned (check_struct_start - transfer_if_valid_struct_start)).
+  Definition check_struct_size := Z.to_nat (bv.unsigned (evaluate_struct_start - check_struct_start)).
+  Definition evaluate_struct_size := Z.to_nat (bv.unsigned (mass_erase_start - evaluate_struct_start)).
+  Definition mass_erase_size := Z.to_nat (bv.unsigned (end_addr - mass_erase_start)).
 
   Definition asn_flag_valid {Σ} : Assertion Σ :=
     asn_ptsto_word ipe_sig_valid_src (low valid_flag) (high valid_flag).
 
-  Definition contract_start_bootcode : BlockVerifierContract :=
+  Definition block_start_bootcode :=
+    [ tst_m R10
+    ; jnz [bv 4] (* check_struct *)
+    ]%list.
+
+  Definition scontract_start_bootcode : BlockVerifierContract :=
     {{
           asn_init_pc start_bootcode_start
         ∗ asn_ipe_registers_init
@@ -119,8 +136,7 @@ Module Bootcode.
         ∗ (asn_ptsto_word saved_ptr byte_zero byte_zero
            ∨ asn_ptsto_word saved_ptr (low isp) (high isp))
     }}
-      [ tst_m R10
-      ; jnz [bv 4] (* check_struct *)]
+      block_start_bootcode
     {{
           R10_reg ↦ saved_ptr
         ∗ asn_ipe_registers_init
@@ -130,7 +146,14 @@ Module Bootcode.
               ∗ asn_fin_pc check_struct_start)
     }}.
 
-  Definition contract_transfer_if_valid_struct : BlockVerifierContract :=
+
+  Definition block_transfer_if_valid_struct :=
+      [ cmp_rm R11 R12
+      ; jnz [bv 0x18] (* end *)
+      ; mov_mm R13 R10
+      ]%list.
+
+  Definition scontract_transfer_if_valid_struct : BlockVerifierContract :=
     {{
           asn_init_pc transfer_if_valid_struct_start
 
@@ -144,9 +167,7 @@ Module Bootcode.
         ∗ asn_ptsto_word ipe_struct_pointer_src (low isp) (high isp)
         ∗ asn_ptsto_word saved_ptr byte_zero byte_zero
     }}
-      [ cmp_rm R11 R12
-      ; jnz [bv 0x7B] (* end *)
-      ; mov_mm R13 R10 ]
+      block_transfer_if_valid_struct
     {{
           asn_fin_pc check_struct_start
 
@@ -161,7 +182,17 @@ Module Bootcode.
         ∗ asn_ptsto_word saved_ptr (low isp) (high isp)
     }}.
 
-  Definition contract_check_struct : BlockVerifierContract :=
+  Definition block_check_struct :=
+      [ mov_mr R10 R6
+      ; mov_rr R15 R14
+      ; xor_ar R6 R14
+      ; xor_ar R6 R14
+      ; xor_ar R6 R14
+      ; cmp_mr R6 R14
+      ; jnz [bv 0xA] (* mass_erase_init *)
+      ]%list.
+
+  Definition scontract_check_struct : BlockVerifierContract :=
     {{
           asn_init_pc check_struct_start
 
@@ -177,14 +208,7 @@ Module Bootcode.
         ∗ asn_ptsto_word (isp +' 4) (term_var "segb1_l") (term_var "segb1_h")
         ∗ asn_ptsto_word (isp +' 6) (term_var "check_l") (term_var "check_h")
     }}
-      [ mov_mr R10 R6
-      ; mov_rr R15 R14
-      ; xor_ar R6 R14
-      ; xor_ar R6 R14
-      ; xor_ar R6 R14
-      ; cmp_mr R6 R14
-      ; jnz [bv 0xA] (* mass_erase_init *)
-      ]
+      block_check_struct
     {{
           ( asn_fin_pc evaluate_struct_start
           ∨ asn_fin_pc mass_erase_start)
@@ -206,7 +230,14 @@ Module Bootcode.
             ; "segb1_l"  :: ty.byteBits; "segb1_h"  :: ty.byteBits
             ; "check_l"  :: ty.byteBits; "check_h"  :: ty.byteBits ].
 
-  Definition contract_evaluate_struct : BlockVerifierContract :=
+  Definition block_evaluate_struct :=
+    [ mov_im R6 (bv.of_Z (-2)%Z) R9
+    ; mov_im R6 (bv.of_Z (-4)%Z) R8
+    ; mov_im R6 (bv.of_Z (-6)%Z) R7
+    ; jump JMP [bv 0x6] (* end *)
+    ]%list.
+
+  Definition scontract_evaluate_struct : BlockVerifierContract :=
     {{
          asn_init_pc evaluate_struct_start
 
@@ -220,10 +251,7 @@ Module Bootcode.
        ∗ asn_ptsto_word (isp +' 2) (low (term_var "segb2")) (high (term_var "segb2"))
        ∗ asn_ptsto_word isp (low (term_var "ipectl")) (high (term_var "ipectl"))
     }}
-      [ mov_im R6 (bv.of_Z (-2)%Z) R9
-      ; mov_im R6 (bv.of_Z (-4)%Z) R8
-      ; mov_im R6 (bv.of_Z (-6)%Z) R7
-      ; jump JMP [bv 0x69] (* end *) ]
+      block_evaluate_struct
     {{
          asn_fin_pc end_addr
 
@@ -241,20 +269,21 @@ Module Bootcode.
        ∗ asn_ptsto_word isp (low (term_var "ipectl")) (high (term_var "ipectl"))
     }} with [ "ipectl" :: ty.wordBits; "segb1" :: ty.wordBits; "segb2" :: ty.wordBits ].
 
-  Lemma valid_start_bootcode : ValidBlockVerifierContract contract_start_bootcode.
+  Lemma valid_start_bootcode : ValidBlockVerifierContract scontract_start_bootcode.
   Proof. now symbolic_simpl. Qed.
 
-  Lemma valid_transfer_if_valid_struct : ValidBlockVerifierContract contract_transfer_if_valid_struct.
+  Lemma valid_transfer_if_valid_struct : ValidBlockVerifierContract scontract_transfer_if_valid_struct.
   Proof. now symbolic_simpl. Qed.
 
-  Lemma valid_check_struct : ValidBlockVerifierContract contract_check_struct.
+  Lemma valid_check_struct : ValidBlockVerifierContract scontract_check_struct.
   Proof. now symbolic_simpl. Qed.
 
-  Lemma valid_evaluate_struct : ValidBlockVerifierContract contract_evaluate_struct.
+  Lemma valid_evaluate_struct : ValidBlockVerifierContract scontract_evaluate_struct.
   Proof.
     symbolic_simpl.
     intuition;
       unfold bv.app; unfold bv.take; unfold bv.drop;
       destruct bv.appView; reflexivity.
   Qed.
-End Bootcode.
+
+End BootcodeBlocks.
