src/verification/Bootcode.v
@@ -1,0 +1,1155 @@
+From Coq Require Import
+  ZArith.ZArith
+  Lists.List
+  Strings.String.
+From Katamaran Require Import
+  Bitvector
+  Notations
+  Specification
+  SmallStep.Step.
+Require Import
+  BlockVer.Spec
+  BlockVer.Verifier
+  IrisModel
+  IrisInstance
+  Machine
+  Sig
+  BootcodeBlocks
+  LoopVerification
+  Contracts.
+
+From iris.base_logic Require lib.gen_heap lib.iprop invariants.
+From iris.bi Require interface big_op.
+From iris.algebra Require dfrac big_op.
+From iris.program_logic Require weakestpre adequacy.
+From iris.proofmode Require string_ident tactics.
+From stdpp Require namespaces.
+Import iris.bi.big_op.
+Import iris.algebra.big_op.
+Import iris.program_logic.weakestpre.
+Import iris.proofmode.tactics.
+
+Open Scope ctx_scope.
+Set Implicit Arguments.
+
+Import ctx.resolution.
+Import ctx.notations.
+Import env.notations.
+Import ListNotations.
+
+Import Contracts.
+Import MSP430BlockVerifShalExecutor.
+Import MSP430BlockVerifSpec.
+Import MSP430IrisAdeqParameters.
+Import MSP430IrisBase.
+Import MSP430IrisInstance.
+Import MSP430Program.
+Import MSP430Semantics.
+Import MicroSail.ShallowExecutor.
+Import SmallStepNotations.
+Import ctx.notations.
+Import ctx.resolution.
+Import env.notations.
+
+Module inv := invariants.
+
+Section Bootcode.
+  Import bv.notations.
+  Import ListNotations.
+  Import TermNotations.
+  Import Spec.Assembly.
+  Import BootcodeBlocks.
+
+  Open Scope hex_Z_scope.
+
+  Ltac iIntros_anon :=
+    iIntros "H"; repeat iDestruct "H" as "[? H]"; iDestruct "H" as "?".
+
+  Definition ipectl : bv 16 := [bv 0xC0]. (* enabled and locked *)
+  Definition segb1 : bv 16 := [bv 0x4] .  (* * 16 = 0x40 *)
+  Definition segb2 : bv 16 := [bv 0x5].   (* * 16 = 0x50 *)
+  Definition data_addr : bv 16 := [bv 0x4A].
+  Definition data_size := Z.to_nat (maxAddr - bv.unsigned (end_addr))%Z.
+
+  Definition inv_fortytwo `{sailGS Σ} : iProp Σ :=
+    interp_ptsto_readonly data_addr [bv 42].
+
+  (* unprotected addresses, excluding bootcode which should be in ROM or smth *)
+  Definition advAddrs1 :=
+    bv.seqBv end_addr (Z.to_nat (bv.unsigned segb1 * 16 - bv.unsigned end_addr))%Z.
+  Definition advAddrs2 :=
+    bv.seqBv (bv.shiftl segb2 [bv [3] 4]) (Z.to_nat (maxAddr - bv.unsigned segb2 * 16))%Z.
+  Definition advAddrs : list _ := advAddrs1 ++ advAddrs2.
+
+  Definition block_mass_erase : list ast_with_args :=
+    [FAIL] ++ repeat (mov_rr CG2 CG2) 5.
+
+  Definition mem_has_word (μ : Memory) (a : Val ty.wordBits) (w : Val ty.wordBits) : Prop :=
+    exists v0 v1, map μ (bv.seqBv a 2) = [v0; v1]%list /\ bv.app v0 v1 = w.
+
+  Definition mem_has_instr (μ : Memory) (a : Val ty.wordBits) (instr : ast) : Prop :=
+    exists w, mem_has_word μ a w /\ pure_decode (Word w) = inr instr.
+
+  Fixpoint mem_has_instrs (μ : Memory) (a : Val ty.wordBits) (instrs : list ast_with_args) : Prop :=
+    match instrs with
+    | instr :: instrs =>
+        mem_has_instr μ a (instr_without_args instr)
+        /\ match instr with
+           | I0 _ =>
+               mem_has_instrs μ (a + [bv 2]) instrs
+           | I1 _ x =>
+               mem_has_word μ (a + [bv 2]) x
+               /\ mem_has_instrs μ (a + [bv 4]) instrs
+           | I2 _ x y =>
+               mem_has_word μ (a + [bv 2]) x
+               /\ mem_has_word μ (a + [bv 4]) y
+               /\ mem_has_instrs μ (a + [bv 6]) instrs
+           end%bv
+    | [] => True
+    end%list.
+
+  Local Notation "r '↦' val" := (reg_pointsTo r val) (at level 70).
+
+  Definition minimal_pre `{sailGS Σ} : iProp Σ :=
+    (∃ v, LastInstructionFetch ↦ v) ∗
+    (∃ v, SRCG1_reg ↦ v) ∗
+    MPUCTL0_reg ↦ [bv 0xA500].
+
+  Definition minimal_post `{sailGS Σ} := minimal_pre.
+
+  Definition make_contract `{sailGS Σ} pre post : iProp Σ :=
+    (minimal_pre ∗ pre) -∗
+    (minimal_post ∗ post -∗ WP_loop) -∗
+    WP_loop.
+
+  Definition ipe_register_init `{sailGS Σ} : iProp Σ :=
+    MPUIPC0_reg ↦ [bv 0]
+    ∗ (∃ v, MPUIPSEGB1_reg ↦ v)
+    ∗ (∃ v, MPUIPSEGB2_reg ↦ v).
+
+  Definition start_bootcode_pre `{sailGS Σ} : iProp Σ :=
+    PC_reg ↦ start_bootcode_start
+    ∗ ptsto_instrs start_bootcode_start block_start_bootcode
+    ∗ ipe_register_init
+    ∗ R10_reg ↦ saved_ptr_bv
+    ∗ (ptsto_word saved_ptr_bv [bv 0]
+       ∨ ptsto_word saved_ptr_bv isp_bv).
+
+  Definition start_bootcode_post `{sailGS Σ} : iProp Σ :=
+    ipe_register_init
+    ∗ ptsto_instrs start_bootcode_start block_start_bootcode
+    ∗ R10_reg ↦ saved_ptr_bv
+    ∗ (ptsto_word saved_ptr_bv [bv 0] ∗ PC_reg ↦ transfer_if_valid_struct_start
+       ∨ ptsto_word saved_ptr_bv isp_bv ∗ PC_reg ↦ check_struct_start).
+
+  Definition contract_start_bootcode `{sailGS Σ} : iProp Σ :=
+    make_contract start_bootcode_pre start_bootcode_post.
+
+  Lemma start_bootcode_verified `{sailGS Σ} : ⊢ contract_start_bootcode.
+  Proof.
+    iIntros "Hpre Hk".
+    iApply (sound_sblock_verification_condition valid_start_bootcode [env]
+              $! start_bootcode_start with "[Hpre] [Hk]").
+    - unfold start_bootcode_pre, minimal_pre. cbn -[ptsto_instrs].
+      iDestruct "Hpre" as "((% & ? & % & ? & ?) & ? & ? & ? & ? & H0)".
+      iFrame.
+      rewrite !bi.sep_True !bi.and_emp.
+      cbv [bv.app bv.fold_right bv.bv_case bv.cons bv.wf_double].
+      iDestruct "H0" as "[H0 | H0]".
+      + iSplitL "". done. iLeft. by iSplitR.
+      + iSplitL "". done. iRight. by iSplitR.
+    - cbn.
+      iIntros (an) "(? & [? ?] & (? & ? & ?) & (? & ? & [((_ & [? _] & [? _]) & -> & _) | ((_ & [? _] & [? _]) & -> & _)]))";
+        iApply ("Hk" with "[-]"); iFrame; [iLeft | iRight]; iFrame.
+  Qed.
+
+  Definition transfer_if_valid_struct_pre `{sailGS Σ} : iProp Σ :=
+    PC_reg ↦ transfer_if_valid_struct_start
+    ∗ ptsto_instrs transfer_if_valid_struct_start block_transfer_if_valid_struct
+
+    ∗ ipe_register_init
+    ∗ R10_reg ↦ saved_ptr_bv
+    ∗ R11_reg ↦ valid_flag_bv
+    ∗ R12_reg ↦ ipe_sig_valid_src_bv
+    ∗ R13_reg ↦ ipe_struct_pointer_src_bv
+
+    ∗ ptsto_word ipe_sig_valid_src_bv valid_flag_bv
+    ∗ ptsto_word ipe_struct_pointer_src_bv isp_bv
+    ∗ ptsto_word saved_ptr_bv [bv 0].
+
+  Definition transfer_if_valid_struct_post `{sailGS Σ} : iProp Σ :=
+    PC_reg ↦ check_struct_start
+    ∗ ptsto_instrs transfer_if_valid_struct_start block_transfer_if_valid_struct
+
+    ∗ ipe_register_init
+    ∗ R10_reg ↦ saved_ptr_bv
+    ∗ R11_reg ↦ valid_flag_bv
+    ∗ R12_reg ↦ ipe_sig_valid_src_bv
+    ∗ R13_reg ↦ ipe_struct_pointer_src_bv
+
+    ∗ ptsto_word ipe_sig_valid_src_bv valid_flag_bv
+    ∗ ptsto_word ipe_struct_pointer_src_bv isp_bv
+    ∗ ptsto_word saved_ptr_bv isp_bv.
+
+  Definition contract_transfer_if_valid_struct `{sailGS Σ} : iProp Σ :=
+    make_contract transfer_if_valid_struct_pre transfer_if_valid_struct_post.
+
+  Lemma transfer_if_valid_struct_verified `{sailGS Σ} : ⊢ contract_transfer_if_valid_struct.
+  Proof.
+    iIntros "Hpre Hk".
+    iApply (sound_sblock_verification_condition valid_transfer_if_valid_struct [env]
+              $! transfer_if_valid_struct_start with "[Hpre] [Hk]").
+    - unfold transfer_if_valid_struct_pre, minimal_pre. cbn -[ptsto_instrs].
+      iDestruct "Hpre" as "((% & ? & % & ? & ?) &? & ? & ? & ? & ? & ? & ? & [? ?] & [? ?] & ? & [? ?])".
+      now iFrame.
+    - cbn.
+      iIntros (an) "(? & (? & ? & ? & ? & _) & (? & ? & ?) & [-> _] & (? & ? & ?) & ? & ? & ? & ? & (? & [? _] & [? _]) & (? & [? _] & [? _]) & (? & [? _] & [? _]))".
+      iApply ("Hk" with "[$]").
+  Qed.
+
+  Definition check_struct_pre `{sailGS Σ} (ipectl segb1 segb2 check : bv 16) : iProp Σ :=
+    PC_reg ↦ check_struct_start
+    ∗ ptsto_instrs check_struct_start block_check_struct
+
+    ∗ ipe_register_init
+    ∗ R10_reg ↦ saved_ptr_bv
+    ∗ R15_reg ↦ [bv 0xFFFF]
+    ∗ (∃ v, R6_reg ↦ v)
+    ∗ (∃ v, R14_reg ↦ v)
+
+    ∗ ptsto_word saved_ptr_bv isp_bv
+
+    ∗ ptsto_word isp_bv ipectl
+    ∗ ptsto_word (isp_bv + [bv 2])%bv segb2
+    ∗ ptsto_word (isp_bv + [bv 4])%bv segb1
+    ∗ ptsto_word (isp_bv + [bv 6])%bv check.
+
+  Definition check_struct_post `{sailGS Σ} (ipectl segb1 segb2 check : bv 16) : iProp Σ :=
+    (PC_reg ↦ evaluate_struct_start
+     ∨ PC_reg ↦ mass_erase_start)
+    ∗ ptsto_instrs check_struct_start block_check_struct
+
+    ∗ ipe_register_init
+    ∗ R10_reg ↦ saved_ptr_bv
+    ∗ R15_reg ↦ [bv 0xFFFF]
+    ∗ R6_reg ↦ (isp_bv + [bv 6])%bv
+    ∗ (∃ v, R14_reg ↦ v)
+
+    ∗ ptsto_word saved_ptr_bv isp_bv
+
+    ∗ ptsto_word isp_bv ipectl
+    ∗ ptsto_word (isp_bv + [bv 2])%bv segb2
+    ∗ ptsto_word (isp_bv + [bv 4])%bv segb1
+    ∗ ptsto_word (isp_bv + [bv 6])%bv check.
+
+  Definition contract_check_struct `{sailGS Σ} (ipectl segb1 segb2 check : bv 16) : iProp Σ :=
+    make_contract
+      (check_struct_pre ipectl segb1 segb2 check)
+      (check_struct_post ipectl segb1 segb2 check).
+
+  Lemma ptstomem_subrange_2 `{sailGS Σ} : forall (a b w : bv 16),
+      b = (a + [bv 1])%bv ->
+      @interp_ptstomem _ _ 2 a w ⊣⊢
+        @interp_ptstomem _ _ 1 a (bv.vector_subrange 0 8 w) ∗
+        @interp_ptstomem _ _ 1 b (bv.vector_subrange 8 8 w).
+  Proof.
+    intros a b w ->.
+    iSplit.
+    - iIntros "Hw".
+      unfold interp_ptstomem.
+      destruct bv.appView.
+      iDestruct "Hw" as "[Hlo Hhi]".
+      iSplitL "Hlo".
+      + unfold bv.vector_subrange.
+        cbn -[bv.appView].
+        rewrite bv.take_app.
+        unfold bv.drop.
+        destruct (bv.appView 0 8 xs).
+        destruct (bv.appView 8 0 ys0).
+        destruct ys0, xs.
+        unfold bv.is_wf in i, i0.
+        destruct bin, bin0;
+          destruct i, i0.
+        rewrite bv.app_nil bv.app_nil_r.
+        cbn. iFrame.
+      + unfold bv.vector_subrange.
+        cbn -[bv.appView].
+        rewrite bv.take_full.
+        rewrite bv.drop_app.
+        destruct bv.appView.
+        rewrite bv.add_comm.
+        iFrame.
+    - iIntros "[Hlo Hhi]".
+      unfold interp_ptstomem.
+      destruct (bv.appView 8 (1 * 8) w).
+      destruct (bv.appView 8 (0 * 8) ys).
+      unfold bv.vector_subrange.
+      cbn -[bv.appView interp_ptsto].
+      rewrite bv.take_app bv.take_full.
+      cbn -[bv.appView interp_ptsto].
+      unfold bv.drop.
+      destruct (bv.appView 0 8 xs), (bv.appView 8 0 ys0).
+      destruct ys0, xs, ys.
+      unfold bv.is_wf in i, i0, i1.
+      destruct bin, bin0, bin1;
+        destruct i, i0, i1.
+      rewrite !bv.app_nil !bv.app_nil_r.
+      cbn -[bv.appView interp_ptsto].
+      rewrite bv.appView_app.
+      destruct (bv.appView 8 0 xs0).
+      destruct ys. unfold bv.is_wf in i. destruct bin; destruct i.
+      rewrite bv.app_nil_r. cbn.
+      rewrite !bi.sep_True bv.add_comm. iFrame.
+  Qed.
+
+  Lemma check_struct_verified `{sailGS Σ} (ipectl segb1 segb2 check : bv 16) :
+    ⊢ contract_check_struct ipectl segb1 segb2 check.
+  Proof.
+    iIntros "Hpre Hk".
+    iApply (sound_sblock_verification_condition valid_check_struct
+              [env]
+               .[("ipectl_l" :: ty.byteBits) ↦ bv.vector_subrange 0 8 ipectl]
+               .[("ipectl_h" :: ty.byteBits) ↦ bv.vector_subrange 8 8 ipectl]
+               .[("segb2_l"  :: ty.byteBits) ↦ bv.vector_subrange 0 8 segb2]
+               .[("segb2_h"  :: ty.byteBits) ↦ bv.vector_subrange 8 8 segb2]
+               .[("segb1_l"  :: ty.byteBits) ↦ bv.vector_subrange 0 8 segb1]
+               .[("segb1_h"  :: ty.byteBits) ↦ bv.vector_subrange 8 8 segb1]
+               .[("check_l"  :: ty.byteBits) ↦ bv.vector_subrange 0 8 check]
+               .[("check_h"  :: ty.byteBits) ↦ bv.vector_subrange 8 8 check]
+              $! check_struct_start with "[Hpre] [Hk]").
+    - unfold check_struct_pre, minimal_pre.
+      cbn -[ptsto_instrs bv.is_wf interp_ptstomem bv.appView].
+      iDestruct "Hpre" as "(A & B & C & D & E & F & G & H & I & J & K & L & M)".
+      iSplitR "B C"; last iFrame.
+      iSplitL "A". iAssumption.
+      iSplitR. done.
+      unfold ipe_register_init.
+      iFrame "D E F G H".
+      iSplitL "I". cbn. rewrite !bi.sep_True. by iFrame.
+      iSplitL "J". simpl (bv.appView 1 15 isp_bv). cbn iota.
+      iSplitR. done.
+      { unfold ptsto_word, bv.app. cbn -[interp_ptstomem].
+        iApply ptstomem_subrange_2; auto. }
+      iSplitL "K". simpl (bv.appView 1 15 (isp_bv + [bv 0x2])%bv). cbn iota.
+      iSplitR. done.
+      { unfold ptsto_word, bv.app. cbn -[interp_ptstomem].
+        iApply ptstomem_subrange_2; auto. }
+      iSplitL "L". simpl (bv.appView 1 15 (isp_bv + [bv 0x4])%bv). cbn iota.
+      iSplitR. done.
+      { unfold ptsto_word, bv.app. cbn -[interp_ptstomem].
+        iApply ptstomem_subrange_2; auto. }
+      iSplitR. simpl (bv.appView 1 15 (isp_bv + [bv 0x6])%bv). cbn iota.
+      iSplit; done.
+      unfold ptsto_word, bv.app. cbn -[interp_ptstomem].
+      iApply ptstomem_subrange_2; done.
+    - cbn -[ptsto_instrs bv.is_wf interp_ptstomem bv.appView].
+      simpl (bv.appView 1 15 _%bv). cbn iota.
+      iIntros (an) "(H0 & H1 & H2 & H3 & H4 & H5 & H6 & H7 & H8 & H9 & H10 & H11 & H12 & H13 & H14 & H15)".
+      iApply ("Hk" with "[-]").
+      iFrame "H2".
+      iSplitL "H0 H3". iDestruct "H3" as "[[-> _] | [-> _]]"; by [iLeft | iRight].
+      iFrame "H1 H4 H5 H6 H7 H8".
+      iSplitL "H9".
+      { iDestruct "H9" as "[_ ?]". iApply ptstomem_subrange_2; auto. }
+      iSplitL "H10".
+      { iDestruct "H10" as "[_ ?]". iApply ptstomem_subrange_2; auto. }
+      iSplitL "H11".
+      { iDestruct "H11" as "[_ ?]". iApply ptstomem_subrange_2; auto. }
+      iSplitL "H12".
+      { iDestruct "H12" as "[_ ?]". iApply ptstomem_subrange_2; auto. }
+      iDestruct "H13" as "[_ ?]". iApply ptstomem_subrange_2; auto.
+      unfold bv.app. cbn -[interp_ptstomem].
+      simpl (bv.cons _ (bv.drop 1 (isp_bv + [bv 0x6]))).
+      iFrame.
+  Qed.
+
+
+  Definition evaluate_struct_pre `{sailGS Σ} (ipectl segb1 segb2 : bv 16) : iProp Σ :=
+    PC_reg ↦ evaluate_struct_start
+    ∗ ptsto_instrs evaluate_struct_start block_evaluate_struct
+
+    ∗ ipe_register_init
+    ∗ R6_reg ↦ (isp_bv + [bv 6])%bv
+    ∗ R7_reg ↦ MPUIPC0_addr_bv
+    ∗ R8_reg ↦ MPUIPSEGB2_addr_bv
+    ∗ R9_reg ↦ MPUIPSEGB1_addr_bv
+
+    ∗ ptsto_word (isp_bv + [bv 4])%bv segb1
+    ∗ ptsto_word (isp_bv + [bv 2])%bv segb2
+    ∗ ptsto_word isp_bv ipectl.
+
+  Definition evaluate_struct_post `{sailGS Σ} (ipectl segb1 segb2 : bv 16) : iProp Σ :=
+    PC_reg ↦ end_addr
+    ∗ ptsto_instrs evaluate_struct_start block_evaluate_struct
+
+    ∗ MPUIPC0_reg    ↦ ipectl
+    ∗ MPUIPSEGB1_reg ↦ segb1
+    ∗ MPUIPSEGB2_reg ↦ segb2
+
+    ∗ R6_reg ↦ (isp_bv + [bv 6])%bv
+    ∗ R7_reg ↦ MPUIPC0_addr_bv
+    ∗ R8_reg ↦ MPUIPSEGB2_addr_bv
+    ∗ R9_reg ↦ MPUIPSEGB1_addr_bv
+
+    ∗ ptsto_word (isp_bv + [bv 4])%bv segb1
+    ∗ ptsto_word (isp_bv + [bv 2])%bv segb2
+    ∗ ptsto_word isp_bv ipectl.
+
+  Definition contract_evaluate_struct `{sailGS Σ} (ipectl segb1 segb2 : bv 16) : iProp Σ :=
+    make_contract
+      (evaluate_struct_pre ipectl segb1 segb2)
+      (evaluate_struct_post ipectl segb1 segb2).
+  
+  Lemma evaluate_struct_verified `{sailGS Σ} (ipectl segb1 segb2 : bv 16) :
+    ⊢ contract_evaluate_struct ipectl segb1 segb2.
+  Proof.
+    iIntros "Hpre Hk".
+    iApply (sound_sblock_verification_condition valid_evaluate_struct
+              [env]
+                .[("ipectl" :: ty.wordBits) ↦ ipectl]
+                .[("segb1"  :: ty.wordBits) ↦ segb1]
+                .[("segb2"  :: ty.wordBits) ↦ segb2]
+              $! evaluate_struct_start with "[Hpre] [Hk]");
+      cbn -[ptsto_instrs bv.is_wf interp_ptstomem bv.appView];
+      simpl (bv.appView 1 15 _). cbn iota.
+
+    - iDestruct "Hpre" as "(H0 & H1 & H2 & H3 & H4 & H5 & H6 & H7 & H8 & H9 & H10)".
+      iSplitR "H1 H2"; last iFrame.
+      iFrame "H0 H5 H6 H7".
+      iSplitR. done.
+      iFrame "H3 H4".
+      iSplitL "H8"; last iSplitL "H9"; (iSplitR; first done);
+        unfold ptsto_word, bv.app; cbn -[interp_ptstomem];
+        by iApply ptstomem_subrange_2.
+    - iIntros (an) "(H0 & H1 & H2 & [-> _] & H4 & H5 & H6 & H7 & H8 & H9 & H10 & H11 & H12 & H13)".
+      iApply ("Hk" with "[-]").
+      iFrame "H2 H0 H1 H4 H5 H6 H7 H8 H9 H10".
+      iSplitL "H11"; last iSplitL "H12";
+        iDestruct select (_)%I as "[_ ?]";
+        by iApply ptstomem_subrange_2.
+  Qed.
+
+  Definition mass_erase_pre `{sailGS Σ} : iProp Σ :=
+    PC_reg ↦ mass_erase_start ∗
+    ptsto_instrs mass_erase_start block_mass_erase ∗
+    ipe_register_init.
+
+  Definition contract_mass_erase `{sailGS Σ} : iProp Σ :=
+    make_contract mass_erase_pre False.
+
+  Section Sym_mass_erase.
+    Import asn.notations.
+    Local Notation "'{{' P '}}' i '{{' Q '}}'" :=
+      (@MkBlockVerifierContract [ctx] P%asn i Q%asn)
+        (at level 90, format "'[v' '{{'  P  '}}' '/'  i '/' '{{'  Q  '}}' ']'").
+
+    Definition scontract_mass_erase : BlockVerifierContract :=
+      {{
+          term_var "a" = term_val ty.Address mass_erase_start ∗
+          MPUIPC0_reg ↦ term_val ty.wordBits [bv 0] ∗
+          ∃ "v", MPUIPSEGB1_reg ↦ term_var "v" ∗
+          ∃ "v", MPUIPSEGB2_reg ↦ term_var "v"
+      }}
+        block_mass_erase
+      {{ ⊥ }}.
+
+    Lemma valid_mass_erase : ValidBlockVerifierContract scontract_mass_erase.
+    Proof. now vm_compute. Qed.
+  End Sym_mass_erase.
+
+
+  Lemma mass_erase_verified `{sailGS Σ} : ⊢ contract_mass_erase.
+    iIntros "Hpre Hk".
+  iApply (sound_sblock_verification_condition valid_mass_erase [env]
+            $! mass_erase_start with "[Hpre] [Hk]").
+  - unfold mass_erase_pre, minimal_pre. cbn -[ptsto_instrs].
+    iDestruct "Hpre" as "((% & ? & % & ? & ?) & ? & ? & ?)".
+    now iFrame.
+  - cbn. by iIntros (an) "(? & ? & ? & % & ?)".
+  Qed.
+
+  Definition registers_not_in_bootcode `{sailGS Σ} : iProp Σ :=
+      (∃ v, SP_reg ↦ v)
+    ∗ (∃ v, SRCG1_reg ↦ v)
+    ∗ (∃ v, CG2_reg ↦ v)
+    ∗ (∃ v, R4_reg ↦ v)
+    ∗ (∃ v, R5_reg ↦ v)
+    ∗ (∃ v, MPUCTL0_reg ↦ v)
+    ∗ (∃ v, MPUCTL1_reg ↦ v)
+    ∗ (∃ v, MPUSEGB2_reg ↦ v)
+    ∗ (∃ v, MPUSEGB1_reg ↦ v)
+    ∗ (∃ v, MPUSAM_reg ↦ v)
+    ∗ (∃ v, LastInstructionFetch ↦ v).
+
+  Lemma evaluate_struct_safe `{sailGS Σ} :
+    ⊢
+      PC_reg ↦ evaluate_struct_start
+
+      ∗ minimal_pre
+
+      ∗ ipe_register_init
+
+      ∗ R6_reg ↦ (isp_bv + [bv 6])%bv
+      ∗ (∃ v, R14_reg ↦ v)
+      ∗ R7_reg ↦ MPUIPC0_addr_bv
+      ∗ R8_reg ↦ MPUIPSEGB2_addr_bv
+      ∗ R9_reg ↦ MPUIPSEGB1_addr_bv
+      ∗ R10_reg ↦ saved_ptr_bv
+      ∗ R11_reg ↦ valid_flag_bv
+      ∗ R12_reg ↦ ipe_sig_valid_src_bv
+      ∗ R13_reg ↦ ipe_struct_pointer_src_bv
+      ∗ R15_reg ↦ [bv 0xFFFF]
+      ∗ registers_not_in_bootcode
+
+      ∗ ptsto_word saved_ptr_bv isp_bv
+      ∗ ptsto_word ipe_sig_valid_src_bv valid_flag_bv
+      ∗ ptsto_word ipe_struct_pointer_src_bv isp_bv
+
+      ∗ ptsto_word isp_bv ipectl
+      ∗ ptsto_word (isp_bv + [bv 2])%bv segb2
+      ∗ ptsto_word (isp_bv + [bv 4])%bv segb1
+      ∗ (∃ check, ptsto_word (isp_bv + [bv 6])%bv check)
+
+      ∗ inv_fortytwo
+      ∗ ptstoSthL advAddrs
+
+      ∗ ptsto_instrs start_bootcode_start block_start_bootcode
+      ∗ ptsto_instrs transfer_if_valid_struct_start block_transfer_if_valid_struct
+      ∗ ptsto_instrs check_struct_start block_check_struct
+      ∗ ptsto_instrs evaluate_struct_start block_evaluate_struct
+      ∗ ptsto_instrs mass_erase_start block_mass_erase
+
+      ∗ (PC_reg ↦ (segb1 + [bv 0x8])%bv -∗ WP_loop)
+
+    -∗ WP_loop.
+  Proof.
+    Local Opaque ptstoSthL ptsto_word.
+    iIntros_anon.
+    iApply (evaluate_struct_verified ipectl segb1 segb2 with "[$]").
+    iIntros_anon.
+    iApply fupd_wp.
+    iAssert (loop_pre end_addr ipectl segb1 segb2) with "[-]" as "?".
+    { do 2 iFrame. auto. }
+    iPoseProof (valid_semTriple_loop $! end_addr ipectl segb1 segb2 with "[$]") as "H".
+    iModIntro. cbn. unfold semWP.
+    iApply (wp_mono with "H"). auto.
+  Qed.
+
+  Lemma mass_erase_safe `{sailGS Σ} :
+    ⊢ minimal_pre ∗
+      PC_reg ↦ mass_erase_start ∗
+      ptsto_instrs mass_erase_start block_mass_erase ∗
+      ipe_register_init
+    -∗ WP_loop.
+  Proof.
+    iIntros.
+    iApply (mass_erase_verified with "[$]").
+    iIntros "[? ?]". done.
+  Qed.
+
+  Lemma check_struct_safe `{sailGS Σ} :
+    ⊢
+      minimal_pre
+
+      ∗ PC_reg ↦ check_struct_start
+
+      ∗ ipe_register_init
+
+      ∗ (∃ v, R6_reg ↦ v)
+      ∗ (∃ v, R14_reg ↦ v)
+      ∗ R7_reg ↦ MPUIPC0_addr_bv
+      ∗ R8_reg ↦ MPUIPSEGB2_addr_bv
+      ∗ R9_reg ↦ MPUIPSEGB1_addr_bv
+      ∗ R10_reg ↦ saved_ptr_bv
+      ∗ R11_reg ↦ valid_flag_bv
+      ∗ R12_reg ↦ ipe_sig_valid_src_bv
+      ∗ R13_reg ↦ ipe_struct_pointer_src_bv
+      ∗ R15_reg ↦ [bv 0xFFFF]
+      ∗ registers_not_in_bootcode
+
+      ∗ ptsto_word saved_ptr_bv isp_bv
+      ∗ ptsto_word ipe_sig_valid_src_bv valid_flag_bv
+      ∗ ptsto_word ipe_struct_pointer_src_bv isp_bv
+
+      ∗ ptsto_word isp_bv ipectl
+      ∗ ptsto_word (isp_bv + [bv 2])%bv segb2
+      ∗ ptsto_word (isp_bv + [bv 4])%bv segb1
+      ∗ (∃ check, ptsto_word (isp_bv + [bv 6])%bv check)
+
+      ∗ ptsto_instrs start_bootcode_start block_start_bootcode
+      ∗ ptsto_instrs transfer_if_valid_struct_start block_transfer_if_valid_struct
+      ∗ ptsto_instrs check_struct_start block_check_struct
+      ∗ ptsto_instrs evaluate_struct_start block_evaluate_struct
+      ∗ ptsto_instrs mass_erase_start block_mass_erase
+
+      ∗ inv_fortytwo
+      ∗ ptstoSthL advAddrs
+
+      ∗ (PC_reg ↦ (segb1 + [bv 0x8])%bv -∗ WP_loop)
+
+    -∗ WP_loop.
+  Proof.
+    Local Opaque ptstoSthL ptsto_word.
+    iIntros "H". do 20 iDestruct "H" as "[? H]". iDestruct "H" as "[[%check ?] H]".
+    repeat iDestruct "H" as "[? H]". iDestruct "H" as "?".
+    iApply (check_struct_verified ipectl segb1 segb2 check with "[$]").
+    iIntros "(? & [? | ?] & H)"; repeat iDestruct "H" as "[? H]"; iDestruct "H" as "?".
+    - iApply (evaluate_struct_safe with "[$]").
+    - iApply (mass_erase_safe with "[$]").
+  Qed.
+
+  Lemma transfer_if_valid_struct_safe `{sailGS Σ} :
+    ⊢
+      minimal_pre
+
+      ∗ PC_reg ↦ transfer_if_valid_struct_start
+
+      ∗ ipe_register_init
+
+      ∗ (∃ v, R6_reg ↦ v)
+      ∗ (∃ v, R14_reg ↦ v)
+      ∗ R7_reg ↦ MPUIPC0_addr_bv
+      ∗ R8_reg ↦ MPUIPSEGB2_addr_bv
+      ∗ R9_reg ↦ MPUIPSEGB1_addr_bv
+      ∗ R10_reg ↦ saved_ptr_bv
+      ∗ R11_reg ↦ valid_flag_bv
+      ∗ R12_reg ↦ ipe_sig_valid_src_bv
+      ∗ R13_reg ↦ ipe_struct_pointer_src_bv
+      ∗ R15_reg ↦ [bv 0xFFFF]
+      ∗ registers_not_in_bootcode
+
+      ∗ ptsto_word saved_ptr_bv [bv 0]
+      ∗ ptsto_word ipe_sig_valid_src_bv valid_flag_bv
+      ∗ ptsto_word ipe_struct_pointer_src_bv isp_bv
+
+      ∗ ptsto_word isp_bv ipectl
+      ∗ ptsto_word (isp_bv + [bv 2])%bv segb2
+      ∗ ptsto_word (isp_bv + [bv 4])%bv segb1
+      ∗ (∃ check, ptsto_word (isp_bv + [bv 6])%bv check)
+
+      ∗ ptsto_instrs start_bootcode_start block_start_bootcode
+      ∗ ptsto_instrs transfer_if_valid_struct_start block_transfer_if_valid_struct
+      ∗ ptsto_instrs check_struct_start block_check_struct
+      ∗ ptsto_instrs evaluate_struct_start block_evaluate_struct
+      ∗ ptsto_instrs mass_erase_start block_mass_erase
+
+      ∗ inv_fortytwo
+      ∗ ptstoSthL advAddrs
+
+      ∗ (PC_reg ↦ (segb1 + [bv 0x8])%bv -∗ WP_loop)
+
+    -∗ WP_loop.
+  Proof.
+    Local Opaque ptstoSthL ptsto_word.
+    iIntros "(H & H0 & H1 & H2 & H3 & H4 & H5 & H6 & H7 & H8 & H9 & H10 & H11 & H12 & H13 & H14 & H15 & H16 & H17 & H18 & H19 & H20 & H21 & H22 & H23 & H24 & H25 & H26 & H27)".
+    iApply (transfer_if_valid_struct_verified with "[$]").
+    iIntros "(H38 & H28 & H29 & H30 & H31 & H32 & H33 & H34 & H35 & H36 & H37)".
+    iApply (check_struct_safe with "[$H38 $H28 $H30 $H2 $H3 $H4 $H5 $H6 $H31 $H32 $H33 $H34 $H11 $H12 $H37 $H35 $H36 $H16 $H17 $H18 $H19 $H20 $H29 $H22 $H23 $H24 $H25 $H26 $H27]").
+  Qed.
+
+  Lemma start_bootcode_safe `{sailGS Σ} :
+    ⊢
+      minimal_pre
+
+      ∗ PC_reg ↦ start_bootcode_start
+
+      ∗ ipe_register_init
+
+      ∗ (∃ v, R6_reg ↦ v)
+      ∗ (∃ v, R14_reg ↦ v)
+      ∗ R7_reg ↦ MPUIPC0_addr_bv
+      ∗ R8_reg ↦ MPUIPSEGB2_addr_bv
+      ∗ R9_reg ↦ MPUIPSEGB1_addr_bv
+      ∗ R10_reg ↦ saved_ptr_bv
+      ∗ R11_reg ↦ valid_flag_bv
+      ∗ R12_reg ↦ ipe_sig_valid_src_bv
+      ∗ R13_reg ↦ ipe_struct_pointer_src_bv
+      ∗ R15_reg ↦ [bv 0xFFFF]
+      ∗ registers_not_in_bootcode
+
+      ∗ (ptsto_word saved_ptr_bv [bv 0]
+         ∨ ptsto_word saved_ptr_bv isp_bv)
+      ∗ ptsto_word ipe_sig_valid_src_bv valid_flag_bv
+      ∗ ptsto_word ipe_struct_pointer_src_bv isp_bv
+
+      ∗ ptsto_word isp_bv ipectl
+      ∗ ptsto_word (isp_bv + [bv 2])%bv segb2
+      ∗ ptsto_word (isp_bv + [bv 4])%bv segb1
+      ∗ (∃ check, ptsto_word (isp_bv + [bv 6])%bv check)
+
+      ∗ ptsto_instrs start_bootcode_start block_start_bootcode
+      ∗ ptsto_instrs transfer_if_valid_struct_start block_transfer_if_valid_struct
+      ∗ ptsto_instrs check_struct_start block_check_struct
+      ∗ ptsto_instrs evaluate_struct_start block_evaluate_struct
+      ∗ ptsto_instrs mass_erase_start block_mass_erase
+
+      ∗ inv_fortytwo
+      ∗ ptstoSthL advAddrs
+
+      ∗ (PC_reg ↦ (segb1 + [bv 0x8])%bv -∗ WP_loop)
+
+    -∗ WP_loop.
+  Proof.
+    Local Opaque ptstoSthL ptsto_word.
+    iIntros "(H33 & H0 & H1 & H2 & H3 & H4 & H5 & H6 & H7 & H8 & H9 & H10 & H11 & H12 & H13 & H14 & H15 & H16 & H17 & H18 & H19 & H20 & H21 & H22 & H23 & H24 & H25 & H26 & H27)".
+    iApply (start_bootcode_verified with "[$]").
+    iIntros "(H34 & H28 & H29 & H30 & [[H31 H32] | [H31 H32]])".
+    - iApply (transfer_if_valid_struct_safe with "[$H34 $H32 $H28 $H2 $H3 $H4 $H5 $H6 $H30 $H8 $H9 $H10 $H11 $H12 $H31 $H14 $H15 $H16 $H17 $H18 $H19 $H29 $H21 $H22 $H23 $H24 $H25 $H26 $H27]").
+    - iApply (check_struct_safe with "[$H34 $H32 $H28 $H2 $H3 $H4 $H5 $H6 $H30 $H8 $H9 $H10 $H11 $H12 $H31 $H14 $H15 $H16 $H17 $H18 $H19 $H29 $H21 $H22 $H23 $H24 $H25 $H26 $H27]").
+  Qed.
+
+  Fixpoint code_size (instrs : list ast_with_args) : nat :=
+    match instrs with
+    | []                 => 0
+    | I0 _     :: instrs => 2 + code_size instrs
+    | I1 _ _   :: instrs => 4 + code_size instrs
+    | I2 _ _ _ :: instrs => 6 + code_size instrs
+    end%list%nat.
+
+  Lemma intro_ptsto_word `{sailGS Σ} v0 v1 (a : bv 16) :
+    interp_ptsto (bv.of_Z (0 + bv.unsigned a)) v0 ∗
+    interp_ptsto (bv.of_Z (1 + bv.unsigned a)) v1
+    ⊢ ptsto_word a (bv.app v0 v1).
+  Proof.
+    iIntros "(Hmema & Hmema1)".
+    Local Transparent ptsto_word.
+    unfold ptsto_word, interp_ptstomem.
+    rewrite ?bv.appView_app.
+    replace (@bv.of_Z 16 (0 + bv.unsigned a)%Z) with a by now rewrite bv.of_Z_unsigned.
+    replace (@bv.of_Z 16 (1 + bv.unsigned a)%Z) with (bv.add bv.one a) by now rewrite <-bv.of_Z_add, bv.of_Z_unsigned.
+    replace v1 with (bv.app v1 bv.nil) by now rewrite (bv.app_nil_r v1).
+    rewrite ?bv.appView_app. rewrite (bv.app_nil_r v1). simpl.
+    now iFrame.
+  Qed.
+
+  Lemma intro_ptsto_word2 `{sailGS Σ} {μ : Memory} {a v : bv 16} :
+    mem_has_word μ a v ->
+    ([∗ list] a' ∈ bv.seqBv a 2, interp_ptsto a' (μ a')) ⊢ ptsto_word a v.
+  Proof.
+    iIntros (Hmhw) "Hmem".
+    destruct Hmhw as (v0 & v1 & Heqμ & Heqv).
+    unfold bv.seqBv, seqZ. change (seq 0 ?x) with [0;1]%list%nat.
+    cbn -[bv.add interp_ptstomem].
+    iDestruct "Hmem" as "(Hmema & Hmema1 & _)".
+    inversion Heqμ; subst.
+    now iApply (intro_ptsto_word with "[$Hmema $Hmema1]").
+  Qed.
+
+  Lemma intro_ptstoSthL `{sailGS Σ} (μ : Memory) (addrs : list (bv 16))  :
+    ([∗ list] a' ∈ addrs, interp_ptsto a' (μ a')) ⊢ ptstoSthL addrs.
+  Proof.
+    Local Transparent ptstoSthL.
+    induction addrs as [|a l]; cbn.
+    - now iIntros "_".
+    - iIntros "[Hmema Hmem]".
+      iSplitL "Hmema".
+      + now iExists (μ a).
+      + now iApply IHl.
+  Qed.
+
+  Lemma intro_ptstoinstr_I `{sailGS Σ} {μ : Memory} {a : bv 16} {instr : ast} :
+    (2 + bv.bin a < bv.exp2 16)%N ->
+    mem_has_instr μ a instr ->
+    ([∗ list] a' ∈ bv.seqBv a 2, interp_ptsto a' (μ a'))
+      ⊢ interp_ptstoinstr a (Base.I instr).
+  Proof.
+    iIntros (Hrep (v & Hmhw & Heq)) "Hmem".
+    iExists v.
+    iSplitL; first iApply intro_ptsto_word2; done.
+  Qed.
+
+  Lemma intro_ptstoinstr_D `{sailGS Σ} {μ : Memory} {a : bv 16} {data} :
+    (2 + bv.bin a < bv.exp2 16)%N ->
+    mem_has_word μ a data ->
+    ([∗ list] a' ∈ bv.seqBv a 2, interp_ptsto a' (μ a'))
+      ⊢ interp_ptstoinstr a (Base.D data).
+  Proof.
+    iIntros.
+    iExists data.
+    iSplitL; first iApply (intro_ptsto_word2 (μ := μ)); auto.
+  Qed.
+
+  Lemma intro_ptsto_instrs `{sailGS Σ} {μ : Memory} {a : bv 16} {instrs : list ast_with_args} :
+    (N.of_nat (code_size instrs) + bv.bin a < bv.exp2 16)%N ->
+    mem_has_instrs μ a instrs ->
+    ([∗ list] a' ∈ bv.seqBv a (code_size instrs), interp_ptsto a' (μ a'))
+      ⊢ ptsto_instrs a instrs.
+  Proof.
+    iIntros (Hrep Hmeminstrs) "Hmem".
+    iInduction instrs as [|instr instrs] "IH" forall (a Hrep Hmeminstrs).
+    - done.
+    - rewrite Nat2N.inj_succ in Hrep.
+      destruct instr;
+        simpl (code_size (_ :: instrs));
+        [ replace (S (S (code_size instrs))) with (2 + code_size instrs)%nat by lia
+        | replace (S (S (S (S (code_size instrs))))) with (4 + code_size instrs)%nat by lia
+        | replace (S (S (S (S (S (S (code_size instrs))))))) with (6 + code_size instrs)%nat by lia ];
+        rewrite bv.seqBv_app big_opL_app;
+        [ destruct Hmeminstrs as [Hinstr Hmeminstrs]
+        | destruct Hmeminstrs as [Hinstr [Hdata Hmeminstrs]]
+        | destruct Hmeminstrs as [Hinstr [Hdata0 [Hdada1 Hmeminstrs]]]];
+        iDestruct "Hmem" as "[Hmema Hmema2]".
+      + assert (N.of_nat (code_size (I0 i :: instrs)) >= 2)%N by (simpl; lia).
+        iSplitL "Hmema".
+        * iApply (intro_ptstoinstr_I with "Hmema"); auto. lia.
+        * iApply ("IH" with "[%] [% //] [-]").
+          -- rewrite bv.bin_add_small;
+               cbn -[N.mul] in *;
+               now Lia.lia.
+          -- now rewrite ?bv.add_assoc.
+      + assert (N.of_nat (code_size (I1 i a0 :: instrs)) >= 4)%N by (simpl; lia).
+        change 4%nat with (2 + 2)%nat at 7.
+        rewrite bv.seqBv_app big_sepL_app.
+        iDestruct "Hmema" as "[HmemI HmemD]".
+        iSplitL "HmemI".
+        * iApply (intro_ptstoinstr_I (μ := μ)); auto. lia.
+        * iSplitL "HmemD".
+          -- iApply (intro_ptstoinstr_D (μ := μ)); auto.
+             rewrite bv.bin_add. simpl.
+             assert (2 + (bv.bin a + 2) `mod` bv.exp2 16 <= 2 + (bv.bin a + 2))%N.
+             { apply N.add_le_mono_l. apply N.Div0.mod_le. }
+             lia.
+          -- iApply ("IH" with "[%] [% //] [-]").
+             ++ rewrite bv.bin_add_small;
+                  cbn -[N.mul] in *;
+                  now Lia.lia.
+             ++ now rewrite ?bv.add_assoc.
+      + assert (N.of_nat (code_size (I2 i a0 b :: instrs)) >= 6)%N by (simpl; lia).
+        change 6%nat with (2 + 2 + 2)%nat at 7.
+        rewrite !bv.seqBv_app !big_sepL_app.
+        iDestruct "Hmema" as "[[HmemI HmemD0] HmemD1]".
+        iSplitL "HmemI".
+        * iApply (intro_ptstoinstr_I (μ := μ)); auto. lia.
+        * iSplitL "HmemD0".
+          -- iApply (intro_ptstoinstr_D (μ := μ)); auto.
+             rewrite bv.bin_add. simpl.
+             assert (2 + (bv.bin a + 2) `mod` bv.exp2 16 <= 2 + (bv.bin a + 2))%N.
+             { apply N.add_le_mono_l. apply N.Div0.mod_le. }
+             lia.
+          -- iSplitL "HmemD1".
+             ++ iApply (intro_ptstoinstr_D (μ := μ)); auto.
+                rewrite bv.bin_add. simpl.
+                assert (2 + (bv.bin a + 4) `mod` bv.exp2 16 <= 2 + (bv.bin a + 4))%N.
+                { apply N.add_le_mono_l. apply N.Div0.mod_le. }
+                lia.
+             ++ iApply ("IH" with "[%] [% //] [-]").
+                ** rewrite bv.bin_add_small;
+                     cbn -[N.mul] in *;
+                     now Lia.lia.
+                ** now rewrite ?bv.add_assoc.
+  Qed.
+
+  Lemma in_seqBv_bounds : forall (s : bv 16) (l : nat) (y : bv 16),
+      (bv.unsigned s + l < 2 ^ 16)%Z ->
+      y ∈ bv.seqBv s l ->
+      (s <=ᵘ y /\ y <ᵘ bv.add s (bv.of_nat l))%bv.
+  Proof.
+    intros s l y Hrep Hy.
+    unfold bv.seqBv in Hy.
+    apply list.elem_of_list_fmap in Hy.
+    destruct Hy as [y' [-> Hy']].
+    apply elem_of_seqZ in Hy'.
+    pose proof (bv.unsigned_bounds s) as H_s_bounds.
+    split.
+    - destruct Hy' as [Hlo Hhi].
+      apply bv.ule_iff_unsigned_le.
+      rewrite bv.unsigned_of_Z.
+      unfold bv.truncz.
+      rewrite Zmod_small.
+      assumption. lia.
+    - destruct Hy' as [Hlo Hhi].
+      apply bv.ult_iff_unsigned_lt.
+      rewrite bv.unsigned_of_Z.
+      unfold bv.truncz.
+      rewrite Zmod_small; last lia.
+      replace (bv.unsigned (s + bv.of_nat l)) with (bv.unsigned s + l)%Z;
+        first assumption.
+      apply (Z.le_lt_add_lt 0 l (bv.unsigned s) (2 ^ 16)) in Hrep as Hsrep; [|lia].
+      rewrite bv.unsigned_add.
+      assert (@bv.unsigned 16 (bv.of_nat l) = l) as ->.
+      { unfold bv.unsigned.
+        rewrite bv.bin_of_nat_small.
+        { apply nat_N_Z. }
+        rewrite Z.add_comm in Hrep.
+        apply (Z.le_lt_add_lt 0 (bv.unsigned s) l (2 ^ 16))
+          in Hrep as Hlrep; lia. }
+      unfold bv.truncz.
+      rewrite Zmod_small; lia.
+  Qed.
+
+  Lemma sub_heap_mapsto_interp_ptsto {Σ : gFunctors} {H : sailGS Σ} {s : bv 16} {e : nat} (μ : Memory):
+    (N.of_nat minAddr <= bv.bin s /\ bv.bin s + (N.of_nat e) <= N.of_nat (minAddr + lenAddr)
+     \/ 0x4200 <= bv.bin s /\ bv.bin s + (N.of_nat e) <= 0x420A
+     \/ 0xFF88 <= bv.bin s /\ bv.bin s + (N.of_nat e) <= 0xFF8C)%N
+    ->
+    ([∗ list] y ∈ bv.seqBv s e, gen_heap.pointsto y (dfrac.DfracOwn 1) (μ y))
+      ⊢ [∗ list] a' ∈ bv.seqBv s e, interp_ptsto a' (μ a').
+  Proof.
+    iIntros ([[Hlo Hhi] | [[Hlo Hhi] | [Hlo Hhi]]]) "Hlist";
+    iApply (big_sepL_mono with "Hlist"); intros ? ? Hsom; cbn;
+    iIntros "$"; iPureIntro;
+    apply elem_of_list_lookup_2 in Hsom;
+    unfold MSP430IrisInstance.is_mpu_reg_addr; intro;
+    unfold minAddr, lenAddr in *; cbn in Hhi;
+    apply in_seqBv_bounds in Hsom.
+    - assert (bv.ult [bv [16] 0x5a0] (bv.of_nat 200))%bv by solve_bv.
+      by compute in H1.
+    - solve_bv.
+    - assert (bv.ule (bv.of_N 16896) s)%bv by solve_bv.
+      assert (bv.ule (bv.of_N 16896) [bv [16] 0x5b0])%bv by solve_bv.
+      by compute in H2.
+    - solve_bv.
+    - assert (bv.ule (bv.of_N 65416) s)%bv by solve_bv.
+      assert (bv.ule (bv.of_N 65416) [bv [16] 0x5b0])%bv by solve_bv.
+      by compute in H2.
+    - solve_bv.
+Qed.
+
+  Lemma liveAddrs_split :
+    liveAddrs =
+      (bv.seqBv start_bootcode_start start_bootcode_size
+      ++ bv.seqBv transfer_if_valid_struct_start transfer_if_valid_struct_size
+      ++ bv.seqBv check_struct_start check_struct_size
+      ++ bv.seqBv evaluate_struct_start evaluate_struct_size
+      ++ bv.seqBv mass_erase_start mass_erase_size
+      ++ advAddrs1
+      ++ bv.seqBv (bv.shiftl segb1 [bv [3] 4]) (Z.to_nat (bv.unsigned data_addr - bv.unsigned segb1 * 16))
+      ++ [data_addr]
+      ++ bv.seqBv (data_addr + [bv 1]) (Z.to_nat (bv.unsigned segb2 * 16 - bv.unsigned data_addr - 1))
+      ++ advAddrs2
+      ++ bv.seqBv saved_ptr_bv 2
+      ++ bv.seqBv isp_bv 2
+      ++ bv.seqBv (isp_bv + [bv 2]) 2
+      ++ bv.seqBv (isp_bv + [bv 4]) 2
+      ++ bv.seqBv (isp_bv + [bv 6]) 2
+      ++ bv.seqBv ipe_sig_valid_src_bv 2
+      ++ bv.seqBv ipe_struct_pointer_src_bv 2)%list.
+  Proof. now compute. Qed.
+
+  Lemma bootcode_splitMemory `{sailGS Σ} {μ : Memory} :
+    mem_has_instrs μ start_bootcode_start block_start_bootcode ->
+    mem_has_instrs μ transfer_if_valid_struct_start block_transfer_if_valid_struct ->
+    mem_has_instrs μ check_struct_start block_check_struct ->
+    mem_has_instrs μ evaluate_struct_start block_evaluate_struct ->
+    mem_has_instrs μ mass_erase_start block_mass_erase ->
+
+    (mem_has_word μ saved_ptr_bv [bv 0]
+     \/ mem_has_word μ saved_ptr_bv isp_bv) ->
+    mem_has_word μ ipe_sig_valid_src_bv valid_flag_bv ->
+    mem_has_word μ ipe_struct_pointer_src_bv isp_bv ->
+
+    mem_has_word μ isp_bv ipectl ->
+    mem_has_word μ (isp_bv + [bv 2])%bv segb2 ->
+    mem_has_word μ (isp_bv + [bv 4])%bv segb1 ->
+
+    μ data_addr = [bv 42] ->
+
+    @mem_res _ sailGS_memGS μ ⊢
+      |={⊤}=>
+          ptsto_instrs start_bootcode_start block_start_bootcode ∗
+          ptsto_instrs transfer_if_valid_struct_start block_transfer_if_valid_struct ∗
+          ptsto_instrs check_struct_start block_check_struct ∗
+          ptsto_instrs evaluate_struct_start block_evaluate_struct ∗
+          ptsto_instrs mass_erase_start block_mass_erase ∗
+
+          (ptsto_word saved_ptr_bv [bv 0] ∨ ptsto_word saved_ptr_bv isp_bv) ∗
+          ptsto_word ipe_sig_valid_src_bv valid_flag_bv ∗
+          ptsto_word ipe_struct_pointer_src_bv isp_bv ∗
+
+          ptsto_word isp_bv ipectl ∗
+          ptsto_word (isp_bv + [bv 2])%bv segb2 ∗
+          ptsto_word (isp_bv + [bv 4])%bv segb1 ∗
+          (∃ check, ptsto_word (isp_bv + [bv 6])%bv check) ∗
+
+          inv_fortytwo ∗
+          ptstoSthL advAddrs.
+  Proof.
+    iIntros (μstart μtransfer μcheck μeval μerase
+               μsaved μvalid μisp μipectl μsegb2 μsegb1 μft) "Hmem".
+    unfold mem_res, initMemMap.
+    rewrite liveAddrs_split.
+    rewrite ?map_app ?list_to_map_app ?big_sepM_union.
+    iDestruct "Hmem" as "(Hstart & Htransfer & Hcheck & Heval & Herase
+                           & Hadv1 & Hipe1 & Hft & Hipe2 & Hadv2 & Hsaved
+                           & Hipectl & Hsegb2 & Hsegb1 & Hcksum
+                           & Hvalid & Hisp)".
+    iSplitL "Hstart".
+    { iApply (intro_ptsto_instrs (μ := μ)); [easy..|].
+      iApply (sub_heap_mapsto_interp_ptsto with "Hstart"); compute; by left. }
+    iSplitL "Htransfer".
+    { iApply (intro_ptsto_instrs (μ := μ)); [easy..|].
+      iApply (sub_heap_mapsto_interp_ptsto with "Htransfer"); compute; by left. }
+    iSplitL "Hcheck".
+    { iApply (intro_ptsto_instrs (μ := μ)); [easy..|].
+      iApply (sub_heap_mapsto_interp_ptsto with "Hcheck"); compute; by left. }
+    iSplitL "Heval".
+    { iApply (intro_ptsto_instrs (μ := μ)); [easy..|].
+      iApply (sub_heap_mapsto_interp_ptsto with "Heval"); compute; by left. }
+    iSplitL "Herase".
+    { iApply (intro_ptsto_instrs (μ := μ)); [easy..|].
+      iApply (sub_heap_mapsto_interp_ptsto with "Herase"); compute; by left. }
+    iSplitL "Hsaved".
+    { destruct μsaved as [μsaved | μsaved];
+        [iLeft | iRight];
+        iApply (intro_ptsto_word2 μsaved);
+        iApply (sub_heap_mapsto_interp_ptsto with "Hsaved");
+        compute; right; by left. }
+    iSplitL "Hvalid".
+    { iApply (intro_ptsto_word2 μvalid).
+      iApply (sub_heap_mapsto_interp_ptsto with "Hvalid");
+        compute. right; by right. }
+    iSplitL "Hisp".
+    { iApply (intro_ptsto_word2 μisp).
+      iApply (sub_heap_mapsto_interp_ptsto with "Hisp");
+        compute; right; by right. }
+    iSplitL "Hipectl".
+    { iApply (intro_ptsto_word2 μipectl).
+      iApply (sub_heap_mapsto_interp_ptsto with "Hipectl");
+        compute; right; by left. }
+    iSplitL "Hsegb2".
+    { iApply (intro_ptsto_word2 μsegb2).
+      iApply (sub_heap_mapsto_interp_ptsto with "Hsegb2");
+        compute; right; by left. }
+    iSplitL "Hsegb1".
+    { iApply (intro_ptsto_word2 μsegb1).
+      iApply (sub_heap_mapsto_interp_ptsto with "Hsegb1");
+        compute; right; by left. }
+    iSplitL "Hcksum".
+    { iExists (bv.app (μ (isp_bv + [bv 6])) (μ (isp_bv + [bv 7])))%bv.
+      assert (mem_has_word μ (isp_bv + [bv 6])
+                (bv.app (μ (isp_bv + [bv 6])) (μ (isp_bv + [bv 7]))))%bv
+        as μcksum
+        by now (exists (μ (isp_bv + [bv 0x6])%bv);
+                exists (μ (isp_bv + [bv 0x7])%bv)).
+      iApply (intro_ptsto_word2 μcksum).
+      iApply (sub_heap_mapsto_interp_ptsto with "Hcksum");
+         compute; right; by left. }
+    iSplitL "Hft".
+    {
+      iAssert (interp_ptsto data_addr [bv 42]) with "[Hft]" as "Hft".
+      { unfold interp_ptsto. simpl.
+        rewrite μft. iDestruct "Hft" as "[Hft _]".
+        iFrame. iPureIntro. now compute. }
+      iMod (inv.inv_alloc boot_inv_ro_ns ⊤ (interp_ptsto data_addr [bv 42]) with "Hft")
+        as "Hinv".
+      now iModIntro.
+    }
+    iApply (intro_ptstoSthL μ).
+    iApply big_sepL_app.
+    iSplitL "Hadv1".
+    - iApply (sub_heap_mapsto_interp_ptsto with "Hadv1"); compute; by left.
+    - iApply (sub_heap_mapsto_interp_ptsto with "Hadv2"); compute; by left.
+  Qed.
+
+  Lemma interp_ptsto_valid `{sailGS Σ} {μ a v} :
+    ⊢ mem_inv _ μ -∗ interp_ptsto a v -∗ ⌜μ a = v⌝.
+  Proof.
+    unfold interp_ptsto, mem_inv.
+    iIntros "(%memmap & Hinv & %link) [Hptsto %Hmpu]".
+    iDestruct (gen_heap.gen_heap_valid with "Hinv Hptsto") as "%x".
+    iPureIntro.
+    now apply (map_Forall_lookup_1 _ _ _ _ link).
+  Qed.
+
+  Lemma bv0_is_nil (x : bv 0) : x = bv.nil.
+  Proof.
+    destruct x as [bin wf].
+    destruct bin; first by apply bv.bin_inj.
+    by exfalso.
+  Qed.
+
+  (*
+  Lemma interp_ptstomem_valid `{sailGS Σ} {μ} {a v : bv 16} :
+    ⊢ mem_inv _ μ -∗ @interp_ptstomem _ _ 2 a v -∗ ⌜mem_has_word μ a v⌝.
+  Proof.
+    iIntros "Hinv Hptstomem".
+    destruct (bv.appView 8 8 v) as [v1 v2].
+    destruct (bv.appView 8 0 v2) as [v2 ?].
+    repeat iExists _.
+    iSplit; last eauto.
+    rewrite !ptstomem_bv_app.
+    iDestruct "Hptstomem" as "(Ha0 & Ha1 & Htail)".
+    iDestruct (interp_ptsto_valid with "Hinv Ha0") as "%Hm0".
+    iDestruct (interp_ptsto_valid with "Hinv Ha1") as "%Hm1".
+    iPureIntro.
+    rewrite (bv0_is_nil ys) bv.app_nil_r.
+    rewrite !bv.seqBv_succ !map_cons.
+    repeat f_equal; auto.
+  Qed.
+   *)
+
+  Lemma bootcode_endToEnd
+    {γ γ' : RegStore} {μ μ' : Memory} {δ δ' : CStore [ctx]} {s' : Stm [ctx] ty.unit} :
+
+    (* TODO require whole machine state *)
+    (forall `{sailGS Σ}, ⊢ (PC_reg ↦ (segb1 + [bv 0x8])%bv -∗ WP_loop) : iProp Σ) ->
+
+    mem_has_instrs μ start_bootcode_start block_start_bootcode ->
+    mem_has_instrs μ transfer_if_valid_struct_start block_transfer_if_valid_struct ->
+    mem_has_instrs μ check_struct_start block_check_struct ->
+    mem_has_instrs μ evaluate_struct_start block_evaluate_struct ->
+    mem_has_instrs μ mass_erase_start block_mass_erase ->
+
+    (mem_has_word μ saved_ptr_bv [bv 0]
+     \/ mem_has_word μ saved_ptr_bv isp_bv) ->
+    mem_has_word μ ipe_sig_valid_src_bv valid_flag_bv ->
+    mem_has_word μ ipe_struct_pointer_src_bv isp_bv ->
+
+    mem_has_word μ isp_bv ipectl ->
+    mem_has_word μ (isp_bv + [bv 2])%bv segb2 ->
+    mem_has_word μ (isp_bv + [bv 4])%bv segb1 ->
+
+    read_register γ PC_reg = start_bootcode_start ->
+    read_register γ MPUIPC0_reg = [bv 0] ->
+
+    (* work around unsupported immediate/absolute addressing *)
+    read_register γ R7_reg = MPUIPC0_addr_bv ->
+    read_register γ R8_reg = MPUIPSEGB2_addr_bv ->
+    read_register γ R9_reg = MPUIPSEGB1_addr_bv ->
+    read_register γ R10_reg = saved_ptr_bv ->
+    read_register γ R11_reg = valid_flag_bv ->
+    read_register γ R12_reg = ipe_sig_valid_src_bv ->
+    read_register γ R13_reg = ipe_struct_pointer_src_bv ->
+    read_register γ R15_reg = [bv 0xFFFF] ->
+
+    μ data_addr = [bv 42] ->
+
+    ⟨ γ, μ, δ, fun_loop ⟩ --->* ⟨ γ', μ', δ', s' ⟩ ->
+
+    μ' data_addr = [bv 42].
+  Proof.
+    intros
+      Htrusted_safe
+      μstart μtransfer μcheck μeval μerase
+      μsaved μvalid μisp
+      μipectl μsegb1 μsegb2
+      γpc γipectl
+      γr7 γr8 γr9 γr10 γr11 γr12 γr13 γr15
+      μft
+      steps.
+    refine (adequacy_gen (Q := fun _ _ _ _ => True%I) _ steps _).
+    iIntros (Σ ?).
+    unfold own_regstore.
+    cbn.
+    iIntros "(Hmem & H')".
+    rewrite γpc γipectl γr7 γr8 γr9 γr10 γr11 γr12 γr13 γr15.
+    iMod (bootcode_splitMemory with "Hmem")
+      as "(Hstart & Htransfer & Hcheck & Heval & Herase
+           & Hsaved & Hvalid & Hisp & Hipectl & Hsegb2 & segb1 & Hchksum & #Hft & Hadv)";
+      try assumption.
+    iModIntro.
+    iSplitR "".
+    - destruct (env.view δ).
+      repeat (iDestruct "H'" as "[? H']").
+      iPoseProof (start_bootcode_safe with "[-]") as "H".
+      { Local Opaque ptsto_instrs.
+        iPoseProof Htrusted_safe as "Htrusted_safe".
+        iFrame "∗ #". }
+      iApply (semWP_mono with "H"). by iIntros ([] _) "_".
+    - iIntros "Hmem".
+      iInv "Hft" as ">Hptsto" "_".
+      iDestruct (interp_ptsto_valid with "Hmem Hptsto") as "$".
+      iApply fupd_mask_intro; first set_solver.
+      now iIntros "_".
+  Qed.
+End Bootcode.
