src/verification/LoopVerification.v
@@ -1,0 +1,111 @@
+From Coq Require Import
+     Lists.List.
+From Katamaran Require Import
+     Bitvector
+     Environment
+     Iris.Instance
+     Iris.Base
+     Program
+     Semantics
+     Sep.Hoare
+     Specification
+     MicroSail.ShallowExecutor
+     MicroSail.ShallowSoundness
+     MicroSail.RefineExecutor
+     MicroSail.Soundness.
+
+Require Import
+     Machine
+     Sig
+     IrisModel
+     IrisInstance
+     Model
+     Contracts.
+
+From iris.base_logic Require lib.gen_heap lib.iprop.
+From iris.base_logic Require Export invariants.
+From iris.bi Require interface big_op.
+From iris.algebra Require dfrac.
+From iris.program_logic Require Import weakestpre adequacy.
+From iris.proofmode Require Import string_ident tactics.
+
+Set Implicit Arguments.
+Import ListNotations.
+Import MSP430Specification.
+Import MSP430Program.
+Import MSP430IrisBase.
+Import MSP430IrisInstance.
+Import MSP430Model.
+(* Import MSP430ValidContracts. *)
+
+Import MSP430Signature.
+Module Import MSP430ShallowExecutor :=
+  MakeShallowExecutor MSP430Base MSP430Signature MSP430Program MSP430Specification.
+
+Module Import MSP430ShallowSoundness := MakeShallowSoundness MSP430Base MSP430Signature MSP430Program MSP430Specification MSP430ShallowExecutor MSP430ProgramLogic.
+
+Module Import MSP430Symbolic := MakeSymbolicSoundness MSP430Base MSP430Signature MSP430Program MSP430Specification MSP430ShallowExecutor MSP430Executor.
+
+Section Loop.
+  Context `{sg : sailGS Σ}.
+
+  Local Notation "r '↦' val" := (reg_pointsTo r val) (at level 70).
+  Local Opaque liveAddrs.
+
+  Import bv.notations.
+  Compute bv.eqb (bv.drop 6 [bv [16] 0xC0]) [bv 0x3].
+
+  Definition own_registers : iProp Σ :=
+      (∃ v, SP_reg ↦ v)
+    ∗ (∃ v, SRCG1_reg ↦ v)
+    ∗ (∃ v, CG2_reg ↦ v)
+    ∗ (∃ v, R4_reg ↦ v)
+    ∗ (∃ v, R5_reg ↦ v)
+    ∗ (∃ v, R6_reg ↦ v)
+    ∗ (∃ v, R7_reg ↦ v)
+    ∗ (∃ v, R8_reg ↦ v)
+    ∗ (∃ v, R9_reg ↦ v)
+    ∗ (∃ v, R10_reg ↦ v)
+    ∗ (∃ v, R11_reg ↦ v)
+    ∗ (∃ v, R12_reg ↦ v)
+    ∗ (∃ v, R13_reg ↦ v)
+    ∗ (∃ v, R14_reg ↦ v)
+    ∗ (∃ v, R15_reg ↦ v)
+    ∗ (∃ v, MPUCTL0_reg ↦ v)
+    ∗ (∃ v, MPUCTL1_reg ↦ v)
+    ∗ (∃ v, MPUSEGB2_reg ↦ v)
+    ∗ (∃ v, MPUSEGB1_reg ↦ v)
+    ∗ (∃ v, MPUSAM_reg ↦ v)
+    ∗ (∃ v, LastInstructionFetch ↦ v).
+
+  Definition loop_pre (pc ipectl segb1 segb2 : bv 16) : iProp Σ :=
+      PC_reg         ↦ pc
+    ∗ MPUIPC0_reg    ↦ ipectl
+    ∗ MPUIPSEGB1_reg ↦ segb1
+    ∗ MPUIPSEGB2_reg ↦ segb2
+
+    (* ipe configured *)
+    ∗ ⌜bv.drop 6 ipectl = [bv 0x3]⌝
+    ∗ ⌜bv.ult segb1 segb2⌝
+
+    (* pc untrusted *)
+    ∗ (⌜(bv.unsigned pc < bv.unsigned segb1 * 16)%Z⌝
+       ∨ ⌜(bv.unsigned segb2 * 16 <= bv.unsigned pc)%Z⌝)
+
+    (* TODO *)
+    (* ∗ asn_accessible_addresses "segb1" "segb2" *)
+
+    ∗ own_registers
+
+    ∗ ▷ (PC_reg ↦ segb1 + [bv 8] -∗ WP_loop).
+
+  Definition semTriple_loop : iProp Σ :=
+    (∀ pc ipectl segb1 segb2,
+        semTriple env.nil
+          (loop_pre pc ipectl segb1 segb2)
+          (FunDef loop)
+          (fun _ _ => True))%I.
+
+  Lemma valid_semTriple_loop : ⊢ semTriple_loop.
+  Admitted.
+End Loop.
