src/verification/Model.v
@@ -1,0 +1,58 @@
+From Coq Require Import
+     Program.Tactics
+     Lists.List.
+From Katamaran Require Import
+     Bitvector
+     Environment
+     Iris.Instance
+     Iris.Base
+     Program
+     Semantics
+     Sep.Hoare
+     Specification.
+
+Require Import
+     Machine
+     Contracts
+     IrisModel
+     IrisInstance
+     Sig.
+
+From Equations Require Import
+     Equations.
+
+From iris.base_logic Require lib.gen_heap lib.iprop.
+From iris.base_logic Require Export invariants.
+From iris.bi Require interface big_op.
+From iris.algebra Require dfrac.
+From iris.program_logic Require Import weakestpre total_weakestpre adequacy.
+From iris.program_logic Require lifting.
+From iris.program_logic Require total_lifting.
+From iris.proofmode Require Import string_ident tactics.
+
+Set Implicit Arguments.
+Import ListNotations.
+Import bv.notations.
+
+Import MSP430Program.
+Import MSP430Signature.
+
+Import MSP430IrisBase.
+Import MSP430IrisInstance.
+
+Module MSP430Model.
+  Import MSP430Signature.
+  Import MSP430Specification.
+  Import MSP430Program.
+
+  Module MSP430ProgramLogic <: ProgramLogicOn MSP430Base MSP430Signature MSP430Program MSP430Specification.
+    Include ProgramLogicOn MSP430Base MSP430Signature MSP430Program MSP430Specification.
+  End MSP430ProgramLogic.
+  Include MSP430ProgramLogic.
+
+  Include IrisInstanceWithContracts MSP430Base MSP430Signature
+    MSP430Program MSP430Semantics MSP430Specification MSP430IrisBase
+    MSP430IrisAdeqParameters MSP430IrisInstance.
+
+  (* proofs of lemmas and foreign functions... *)
+End MSP430Model.
